coq/Parser_sound.v
@@ -1,6 +1,9 @@
-Require Import Arith List.
+Require Import Arith Bool List.
 Require Import GallStar.Defs.
 Require Import GallStar.Lex.
+Require Import GallStar.Prediction.
+Require Import GallStar.Prediction_error_free.
+Require Import GallStar.Prediction_complete.
 Require Import GallStar.Parser.
 Require Import GallStar.Tactics.
 Require Import GallStar.Termination.
@@ -57,7 +60,8 @@ Proof.
   intros; eapply multistep_sound'; eauto.
 Qed.
 
-Theorem parser_sound :
+(* This is the original, weaker version of soundness *)
+Theorem parse_sound :
   forall (g  : grammar)
          (ss : list symbol)
          (ts : list token)
@@ -71,4 +75,926 @@ Proof.
   - constructor. (* how do I get auto to take care of this? *)
   - apply stack_prefix_derivation_init. 
 Qed.
-  
+
+(* The stronger parser soundness theorems -- one for unique derivations, one for
+   ambiguous derivations, appear below. *)
+
+Definition unprocTailSyms' (frs : list frame) :=
+  unprocTailSyms (map loc frs).
+
+(* Invariant for proving the "unambiguous" version of the parser soundness
+   lemma. The processed stack symbols and the semantic values stored
+   in each frame comprise a unique partial derivation for the tokens that
+   have been consumed. *)
+Inductive unique_frames_derivation (g : grammar) :
+  list frame -> list token -> list token -> Prop :=
+| USD_empty :
+    forall w,
+      unique_frames_derivation g [] [] w
+| USD_bottom :
+    forall o pre suf v wpre wsuf,
+      gamma_derivation g pre wpre v
+      -> (forall wpre' wsuf' v',
+             wpre' ++ wsuf' = wpre ++ wsuf
+             -> gamma_derivation g pre wpre' v'
+             -> gamma_recognize g suf wsuf'
+             -> wpre' = wpre /\ wsuf' = wsuf /\ v' = v)
+      -> unique_frames_derivation g [Fr (Loc o pre suf) v] wpre wsuf
+| USD_upper :
+    forall cr ce o o' pre pre' x suf suf' frs wpre wmid wsuf v v',
+      cr = Fr (Loc o pre (NT x :: suf)) v
+      -> ce = Fr (Loc o' pre' suf') v'
+      -> unique_frames_derivation g (cr :: frs) wpre (wmid ++ wsuf)
+      -> gamma_derivation g pre' wmid v'
+      -> (forall wmid' wsuf' v'',
+             wmid' ++ wsuf' = wmid ++ wsuf
+             -> gamma_derivation g pre' wmid' v''
+             -> gamma_recognize g (suf' ++ suf ++ unprocTailSyms' frs) wsuf'
+             -> wmid' = wmid /\ wsuf' = wsuf /\ v'' = v')
+      (* Here's the interesting part -- all pushes are unique *)
+      -> (forall rhs,
+             In (x, rhs) g
+             -> gamma_recognize g (rhs ++ suf ++ unprocTailSyms' frs) (wmid ++ wsuf)
+             -> rhs = pre' ++ suf')
+      -> unique_frames_derivation g (ce :: cr :: frs) (wpre ++ wmid) wsuf.
+
+Lemma return_preserves_unique_frames_derivation :
+  forall g ce cr cr' frs x o o' pre pre' suf' wpre wsuf v v',
+    ce  = Fr (Loc o pre []) v
+    -> cr  = Fr (Loc o' pre' (NT x :: suf')) v'
+    -> cr' = Fr (Loc o' (pre' ++ [NT x]) suf') (v' ++ [Node x v])
+    -> stack_wf g (ce, cr :: frs)
+    -> unique_frames_derivation g (ce :: cr :: frs) wpre wsuf
+    -> unique_frames_derivation g (cr' :: frs) wpre wsuf.
+Proof.
+  intros g ce cr cr' frs x o o' pre pre' suf' wpre wsuf v v'
+         ? ? ? hw hu; subst; sis.
+  inversion hu as [ ?
+                  | ? ? ? ? ? ? ? ?
+                  | ? ? ? ? ? ? ? ? ? ? ? ? ? ? ?
+                    heq heq' htl hg hder hpush]; subst; clear hu.
+  inv heq; inv heq'.
+  destruct frs.
+  - inv htl.
+    apply USD_bottom.
+    + apply gamma_derivation_app; auto.
+      inv hw; rewrite app_nil_r in *.
+      rew_nil_r wmid; eauto.
+    + intros wpre' wsuf' v' heq hd hr; subst; sis.
+      apply gamma_derivation_split in hd.
+      destruct hd as [w [w' [vs [vs' [? [? [hd hd']]]]]]]; subst.
+      repeat rewrite <- app_assoc in heq.
+      inv hd'.
+      inv H4. rewrite app_nil_r in *.
+      inv H1.
+      eapply H6 in heq; eauto.
+      * destruct heq as [? [? ?]]; subst.
+        assert (ys = pre'0).
+        { rewrite <- H1 in hpush.
+          apply hpush in H0; auto.
+          - rewrite app_nil_r in *; subst; auto.
+          - apply gamma_recognize_app; auto.
+            eapply gamma_derivation__gamma_recognize; eauto. }
+        subst.
+        eapply hder with (v'' := sts) in H1; eauto.
+        destruct H1 as [? [? ?]]; subst.
+        repeat split; auto.
+      * econstructor; eauto.
+        econstructor; eauto.
+        eapply gamma_derivation__gamma_recognize; eauto.
+  - inv htl.
+    inv H3.
+    rewrite <- app_assoc.
+    eapply USD_upper; eauto.
+    + rewrite <- app_assoc; auto.
+    + eapply gamma_derivation_app; auto.
+      inv hw. rewrite app_nil_r in *.
+      rew_nil_r wmid; eauto.
+    + intros wpre' wsuf' v'' heq hd hr; subst; sis.
+      apply gamma_derivation_split in hd.
+      destruct hd as [w [w' [vs [vs' [? [? [hd hd']]]]]]]; subst.
+      repeat rewrite <- app_assoc in heq.
+      inv hd'.
+      inv H6. rewrite app_nil_r in *.
+      inv H1.
+      eapply H8 in heq; eauto.
+      * destruct heq as [? [? ?]]; subst.
+        assert (ys = pre'0).
+        { rewrite <- H1 in hpush.
+          apply hpush in H0; auto.
+          unfold unprocTailSyms'. simpl.
+          apply gamma_recognize_app; auto.
+          eapply gamma_derivation__gamma_recognize; eauto. }
+        subst.
+        eapply hder with (v'' := sts) in H1; eauto.
+        destruct H1 as [? [? ?]]; subst.
+        repeat split; auto.
+      * constructor; auto.
+        econstructor; eauto.
+        eapply gamma_derivation__gamma_recognize; eauto.
+    + intros rhs hi hr; subst.
+      apply H9 in hi; auto.
+      * rewrite hi. apps.
+      * rewrite <- app_assoc in hr; auto.
+Qed.
+
+Lemma consume_preserves_unique_frames_derivation :
+  forall g fr fr' frs o pre a suf v l wpre wsuf,
+    fr = Fr (Loc o pre (T a :: suf)) v
+    -> fr' = Fr (Loc o (pre ++ [T a]) suf) (v ++ [Leaf a l])
+    -> unique_frames_derivation g (fr :: frs) wpre ((a,l) :: wsuf)
+    -> unique_frames_derivation g (fr' :: frs) (wpre ++ [(a,l)]) wsuf.
+Proof.
+  intros g fr fr' frs o pre a suf v l wpre wsuf ? ? hu; subst.
+  inv hu.
+  - constructor.
+    + apply gamma_derivation_app; auto.
+      assert ([(a,l)] = [(a,l)] ++ []) by apps.
+      rewrite H; eauto.
+    + intros wpre' wsuf' v' heq hd hr; subst.
+      apply gamma_derivation_split in hd.
+      destruct hd as [w [w' [v'' [v''' [? [? [hd hd']]]]]]]; subst.
+      inv hd'.
+      inv H1. inv H4. rewrite app_nil_r in*.
+      repeat rewrite <- app_assoc in heq.
+      eapply H7 in heq; eauto.
+      destruct heq as [? [? ?]]; subst.
+      inv H0. repeat split; auto.
+  - inv H2.
+    rewrite <- app_assoc.
+    econstructor; eauto.
+    + rewrite <- app_assoc; auto.
+    + apply gamma_derivation_app; auto.
+      assert ([(a,l)] = [(a,l)] ++ []) by apps.
+      rewrite H; eauto.
+    + intros wpre' wsuf' v'' heq hd hr; subst.
+      apply gamma_derivation_split in hd.
+      destruct hd as [w [w' [v''' [v'''' [? [? [hd hd']]]]]]]; subst.
+      inv hd'.
+      inv H1. inv H7. rewrite app_nil_r in*.
+      repeat rewrite <- app_assoc in heq.
+      eapply H5 in heq; eauto.
+      * destruct heq as [? [? ?]]; subst.
+        inv H0. repeat split; auto.
+      * constructor; auto.
+    + intros rhs hi hr.
+      sis.
+      eapply H8 in hi; eauto.
+      * rewrite hi. apps.
+      * rewrite <- app_assoc in hr; auto.
+Qed.
+
+Lemma push_succ_preserves_usd :
+  forall g fr o pre x suf v frs wpre wsuf rhs,
+    fr = Fr (Loc o pre (NT x :: suf)) v
+    -> no_left_recursion g
+    -> stack_wf g (fr, frs)
+    -> llPredict g x (lstackOf (fr, frs)) wsuf = PredSucc rhs
+    -> unique_frames_derivation g (fr :: frs) wpre wsuf
+    -> unique_frames_derivation g (Fr (Loc (Some x) [] rhs) [] :: fr :: frs) wpre wsuf.
+Proof.
+  intros g fr o pre x suf v frs wpre wsuf rhs ? hn hw hl hu; subst; sis.
+  assert (wpre = wpre ++ []) by apps. rewrite H.
+  econstructor; eauto.
+  - intros wmid' wsuf' v'' heq hd hr; sis; subst.
+    inv hd; auto.
+  - intros rhs' hi hr; sis.
+    eapply llPredict_succ_at_most_one_rhs_applies in hl; eauto.
+Qed.    
+
+Definition unique_prefix_derivation g w st :=
+  match st with
+  | Pst _ (fr, frs) wsuf u =>
+    u = true
+    -> exists wpre,
+        w = wpre ++ wsuf
+        /\ unique_frames_derivation g (fr :: frs) wpre wsuf
+  end.
+
+Lemma step_preserves_upd :
+  forall g w st st',
+    no_left_recursion g
+    -> stack_wf g (Parser.stack st)
+    -> unique_prefix_derivation g w st
+    -> step g st = StepK st'
+    -> unique_prefix_derivation g w st'.
+Proof.
+  intros g w [av (fr,frs) wsuf u] [av' (fr',frs') wsuf' u'] hn hw hu hs.
+  red; red in hu.
+  intros hu'.
+  unfold step in hs; dmeqs h; inv hs; tc;
+  destruct hu as [wpre [heq hu]]; subst; auto.
+  - exists wpre; split; auto.
+    eapply return_preserves_unique_frames_derivation; eauto.
+  - exists (wpre ++ [(t,l1)]); split.
+    + apps.
+    + eapply consume_preserves_unique_frames_derivation; eauto.
+  - exists wpre; split; auto.
+    eapply push_succ_preserves_usd; eauto.
+Qed.
+
+Lemma upd_starts_true :
+  forall g ys ts,
+    unique_prefix_derivation g ts (mkInitState g ys ts).
+Proof.
+  intros g ys ts.
+  unfold mkInitState; sis.
+  intros _.
+  exists []; split; auto.
+  constructor; auto.
+  intros wpre' wsuf' v' heq hd hr; sis.
+  inv hd; auto.
+Qed.
+
+Lemma multistep_sound_unambig' :
+  forall (g      : grammar)
+         (tri    : nat * nat * nat)
+         (a      : Acc lex_nat_triple tri)
+         (w wsuf : list token)
+         (av     : NtSet.t)
+         (stk    : parser_stack)
+         (u      : bool)
+         (a'     : Acc lex_nat_triple (Parser.meas g (Pst av stk wsuf u)))
+         (v      : forest),
+    tri = Parser.meas g (Pst av stk wsuf u)
+    -> no_left_recursion g
+    -> stack_wf g stk
+    -> unique_prefix_derivation g w (Pst av stk wsuf u)
+    -> multistep g (Pst av stk wsuf u) a' = Accept v
+    -> gamma_derivation g (bottomFrameSyms stk) w v
+       /\ (forall v',
+              gamma_derivation g (bottomFrameSyms stk) w v'
+              -> v' = v).
+Proof.
+  intros g tri a.
+  induction a as [tri hlt IH].
+  intros w wsuf av stk u a' v heq hn hw hi hm; subst.
+  apply multistep_accept_cases in hm.
+  destruct hm as [[hf hu] | he].
+  - simpl in hu; subst.
+    apply step_StepAccept_facts in hf.
+    destruct hf as [[xo [rpre [v' [heq]]]] heq']; subst.
+    unfold bottomFrameSyms; simpl; rewrite app_nil_r.
+    red in hi.
+    destruct hi as [wpre [heq hu]]; subst; auto.
+    inv hu.
+    rewrite app_nil_r in *.
+    split; auto.
+    intros v' hd.
+    eapply H6 in hd; eauto.
+    + destruct hd as [? [? ?]]; auto.
+    + apps.
+  - destruct he as [st' [a'' [hf hm]]].
+    destruct st' as [av' stk' wsuf'].
+    eapply IH with (w := w) in hm; eauto. 
+    + erewrite step_preserves_bottomFrameSyms_invar; eauto.
+    + apply step_meas_lt; auto.
+    + eapply step_preserves_stack_wf_invar; eauto.
+    + eapply step_preserves_upd; eauto.
+      simpl; auto.
+Qed.
+
+Lemma multistep_sound_unambig :
+  forall (g      : grammar)
+         (w wsuf : list token)
+         (av     : NtSet.t)
+         (stk    : parser_stack)
+         (u      : bool)
+         (a      : Acc lex_nat_triple (Parser.meas g (Pst av stk wsuf u)))
+         (v      : forest),
+    no_left_recursion g
+    -> stack_wf g stk
+    -> unique_prefix_derivation g w (Pst av stk wsuf u)
+    -> multistep g (Pst av stk wsuf u) a = Accept v
+    -> gamma_derivation g (bottomFrameSyms stk) w v
+       /\ (forall v',
+              gamma_derivation g (bottomFrameSyms stk) w v'
+              -> v' = v).
+Proof.
+  intros; eapply multistep_sound_unambig'; eauto.
+Qed.
+
+Theorem parse_sound_unambig :
+  forall (g  : grammar)
+         (ys : list symbol)
+         (ts : list token)
+         (v  : forest),
+    no_left_recursion g
+    -> parse g ys ts = Accept v
+    -> gamma_derivation g ys ts v
+       /\ (forall v',
+              gamma_derivation g ys ts v'
+              -> v' = v).
+Proof.
+  intros g ys ts v hn hp.
+  unfold parse in hp.
+  eapply multistep_sound_unambig in hp; eauto.
+  - constructor.
+  - apply upd_starts_true.
+Qed.
+
+(* now for the ambiguous case *)
+
+Inductive frames_derivation (g : grammar) :
+  list frame -> list token -> list token -> Prop :=
+| FD_nil  :
+    forall wsuf,
+      frames_derivation g [] [] wsuf
+| FD_cons :
+    forall o pre suf v frs wpre wmid wsuf,
+      gamma_derivation g pre wmid v
+    -> frames_derivation g frs wpre (wmid ++ wsuf) 
+    -> frames_derivation g (Fr (Loc o pre suf) v :: frs) (wpre ++ wmid) wsuf.
+
+Hint Constructors frames_derivation.
+
+Lemma fd_inv_cons :
+  forall g o pre suf v frs w wsuf,
+    frames_derivation g (Fr (Loc o pre suf) v :: frs) w wsuf
+    -> exists wpre wmid,
+      w = wpre ++ wmid
+      /\ frames_derivation g frs wpre (wmid ++ wsuf)
+      /\ gamma_derivation g pre wmid v.
+Proof.
+  intros g o pre suf v frs w wsuf hf; inv hf; eauto.
+Qed.
+
+Lemma return_preserves_frames_derivation :
+  forall g ce cr cr' o o' pre pre' x suf v v' wpre wsuf frs,
+    ce = Fr (Loc o' pre' []) v'
+    -> cr = Fr (Loc o pre (NT x :: suf)) v
+    -> cr' = Fr (Loc o (pre ++ [NT x]) suf) (v ++ [Node x v'])
+    -> stack_wf g (ce, cr :: frs)
+    -> frames_derivation g (ce :: cr :: frs) wpre wsuf
+    -> frames_derivation g (cr' :: frs) wpre wsuf.
+Proof.
+  intros g ce cr cr' o o' pre pre' x suf v v' w wsuf frs ? ? ? hw hf; subst.
+  apply fd_inv_cons in hf; destruct hf as [w' [wmid' [heq [hf hg']]]]; subst.
+  apply fd_inv_cons in hf; destruct hf as [wpre [wmid [heq [hf hg]]]]; subst.
+  rewrite <- app_assoc; econstructor; eauto.
+  - apply gamma_derivation_app; auto.
+    inv hw; rewrite app_nil_r in *.
+    rew_nil_r wmid'; eauto.
+  - rewrite <- app_assoc; auto.
+Qed.
+
+Lemma consume_preserves_frames_derivation :
+  forall g fr fr' frs o pre suf v a l wpre wsuf,
+    fr = Fr (Loc o pre (T a :: suf)) v
+    -> fr' = Fr (Loc o (pre ++ [T a]) suf) (v ++ [Leaf a l])
+    -> frames_derivation g (fr :: frs) wpre ((a,l) :: wsuf)
+    -> frames_derivation g (fr' :: frs) (wpre ++ [(a,l)]) wsuf.
+Proof.
+  intros g fr fr' frs o pre suf v a l wpre wsuf ? ? hf; subst; inv hf.
+  rewrite <- app_assoc; econstructor.
+  - apply gamma_derivation_app; auto.
+    rew_nil_r [(a,l)]; eauto.
+  - rewrite <- app_assoc; auto.
+Qed.
+
+Lemma push_preserves_frames_derivation :
+  forall g cr ce frs o o' pre suf v x rhs wpre wsuf,
+    cr = Fr (Loc o pre (NT x :: suf)) v
+    -> ce = Fr (Loc o' [] rhs) []
+    -> frames_derivation g (cr :: frs) wpre wsuf
+    -> frames_derivation g (ce :: cr :: frs) wpre wsuf.
+Proof.
+  intros g cr ce frs o o' pre suf v x rhs w wsuf ? ? hf; subst.
+  apply fd_inv_cons in hf; destruct hf as [wpre [wmid [heq [hf hg]]]]; subst.
+  rew_nil_r (wpre ++ wmid); eauto.
+Qed.
+
+Definition frames_prefix_derivation g w st :=
+  match st with
+  | Pst _ (fr, frs) wsuf _ =>
+    exists wpre,
+    w = wpre ++ wsuf
+    /\ frames_derivation g (fr :: frs) wpre wsuf
+  end.
+
+Lemma step_preserves_frames_prefix_derivation :
+  forall g w st st',
+    stack_wf g (Parser.stack st)
+    -> frames_prefix_derivation g w st
+    -> step g st = StepK st'
+    -> frames_prefix_derivation g w st'.
+Proof.
+  intros g w [av (fr,frs) ts u] [av' (fr',frs') ts' u'] hw hf hs.
+  red; red in hf.
+  destruct hf as [wpre [heq hf]]; subst.
+  unfold step in hs; dmeqs h; tc; inv hs.
+  - eexists; split; eauto.
+    eapply return_preserves_frames_derivation; eauto.
+  - exists (wpre ++ [(t,l1)]); split; apps.
+    eapply consume_preserves_frames_derivation; eauto.
+  - eexists; split; eauto.
+    eapply push_preserves_frames_derivation; eauto.
+  - eexists; split; eauto.
+    eapply push_preserves_frames_derivation; eauto.
+Qed.
+
+Lemma trees_eq__gammas_eq_words_eq' :
+  forall g ys w v,
+    gamma_derivation g ys w v
+    -> forall ys' w',
+        gamma_derivation g ys' w' v
+        -> ys' = ys /\ w' = w.
+Proof.
+  intros g ys w v hg.
+  induction hg using gamma_derivation_mutual_ind with
+      (P := fun s w t (hs : sym_derivation g s w t) =>
+              forall s' w',
+                sym_derivation g s' w' t
+                -> s' = s /\ w' = w).
+  - intros s' w' hs; inv hs; auto.
+  - intros s' w' hs; inv hs; firstorder.
+  - intros ys' w' hg; inv hg; auto.
+  - intros ys' w' hg'; inv hg'.
+    apply IHhg in H3; destruct H3; subst.
+    apply IHhg0 in H4; destruct H4; subst; auto.
+Qed.
+
+Lemma trees_eq__gammas_eq_words_eq :
+  forall g ys ys' w w' v,
+    gamma_derivation g ys w v
+    -> gamma_derivation g ys' w' v
+    -> ys' = ys /\ w' = w.
+Proof.
+  intros; eapply trees_eq__gammas_eq_words_eq'; eauto.
+Qed.
+
+(* Invariant for proving the "ambiguous" version of the parser soundness
+   theorem. The processed stack symbols and semantic values constructed
+   for them comprise a correct partial derivation for the tokens consumed,
+   and there exists a different semantic value for a (possibly different)
+   prefix of the complete token sequence. *)
+Inductive ambiguous_frames_derivation (g : grammar) :
+  list frame -> list token -> list token -> Prop :=
+| AFD_push :
+    forall cr ce o o' pre pre' x suf suf' v v' wpre wmid wsuf frs alt_rhs,
+      cr = Fr (Loc o pre (NT x :: suf)) v
+      -> ce = Fr (Loc o' pre' suf') v'
+      -> frames_derivation g (cr :: frs) wpre (wmid ++ wsuf)
+      -> gamma_derivation g pre' wmid v'
+      -> In (x, alt_rhs) g
+      -> pre' ++ suf' <> alt_rhs
+      -> gamma_recognize g (alt_rhs ++ suf ++ unprocTailSyms' frs) (wmid ++ wsuf)
+      -> ambiguous_frames_derivation g (ce :: cr :: frs) (wpre ++ wmid) wsuf
+| AFD_sem :
+    forall fr o pre suf v v' wpre wmid wmid' wsuf wsuf' frs,
+      fr = Fr (Loc o pre suf) v
+      -> frames_derivation g frs wpre (wmid ++ wsuf)
+      -> gamma_derivation g pre wmid v
+      -> gamma_derivation g pre wmid' v'
+      -> gamma_recognize g (suf ++ unprocTailSyms' frs) wsuf'
+      -> wmid' ++ wsuf' = wmid ++ wsuf
+      -> v' <> v
+      -> ambiguous_frames_derivation g (fr :: frs) (wpre ++ wmid) wsuf
+| AFD_tail :
+    forall fr o pre suf v frs wpre wmid wsuf,
+      fr = Fr (Loc o pre suf) v
+      -> ambiguous_frames_derivation g frs wpre (wmid ++ wsuf)
+      -> gamma_derivation g pre wmid v
+      -> ambiguous_frames_derivation g (fr :: frs) (wpre ++ wmid) wsuf.
+
+Lemma return_preserves_ambiguous_frames_derivation :
+  forall g ce cr cr' o o' pre pre' x suf v v' wpre wsuf frs,
+    ce = Fr (Loc o' pre' []) v'
+    -> cr = Fr (Loc o pre (NT x :: suf)) v
+    -> cr' = Fr (Loc o (pre ++ [NT x]) suf) (v ++ [Node x v'])
+    -> stack_wf g (ce, cr :: frs)
+    -> ambiguous_frames_derivation g (ce :: cr :: frs) wpre wsuf
+    -> ambiguous_frames_derivation g (cr' :: frs) wpre wsuf.
+Proof.
+  intros g ce cr cr' o o' pre pre' x suf v v' w wsuf frs ? ? ? hw ha; subst.
+  inv ha; subst.
+  - (* ambig push case *)
+    inv H2; inv H3.
+    rewrite app_nil_r in *; sis.
+    rename pre'0 into rhs; rename pre0 into pre;
+    rename suf0 into suf; rename v0 into v; rename v'0 into v';
+    rename x0 into x.    
+    apply fd_inv_cons in H4.
+    destruct H4 as [wp [wp' [heq [hf hg]]]]; subst.
+    apply gamma_recognize_split in H10.
+    destruct H10 as [w [w' [heq [hr hr']]]]; subst.
+    apply gamma_recognize__exists_gamma_derivation in hr.
+    destruct hr as [v_alt hr].
+    inv hw. rewrite app_nil_r in *.
+    rewrite <- app_assoc.
+    eapply AFD_sem with (v := v ++ [Node x v'])
+                        (v' := v ++ [Node x v_alt])
+                        (wmid' := wp' ++ w); eauto.
+    + rewrite <- app_assoc; auto.
+    + apply gamma_derivation_app; auto.
+      rew_nil_r wmid; eauto.
+    + apply gamma_derivation_app; eauto.
+      rew_nil_r w; eauto.
+    + repeat rewrite <- app_assoc in *.
+      rewrite heq; auto.
+    + unfold not; intros.
+      apply app_inv_head in H.
+      inv H.
+      eapply trees_eq__gammas_eq_words_eq with
+          (ys := rhs) in hr; eauto.
+      firstorder.
+  - (* sem case *)
+    inv H1; inv H2; unfold unprocTailSyms' in *; sis.
+    rewrite <- app_assoc.
+    eapply AFD_sem with (v' := v ++ [Node x v'0])
+                        (wmid' := wmid0 ++ wmid'); eauto.
+    + rewrite <- app_assoc; auto.
+    + apply gamma_derivation_app; auto.
+      inv hw; rewrite app_nil_r in *.
+      rew_nil_r wmid; eauto.
+    + apply gamma_derivation_app; auto.
+      inv hw; rewrite app_nil_r in *.
+      rew_nil_r wmid'; eauto.
+    + repeat rewrite <- app_assoc in *.
+      rewrite H6; auto.
+    + unfold not; intros.
+      apply app_inv_head in H.
+      inv H; tc.
+  - (* tail case *)
+    inv H1.
+    inv H2.
+    + (* caller push case *)
+      inv H3.
+      rewrite <- app_assoc.
+      eapply AFD_push; eauto.
+      * rewrite <- app_assoc; auto.
+      * apply gamma_derivation_app; auto.
+        inv hw. inv H14; rewrite app_nil_r in *.
+        rew_nil_r wmid; eauto.
+      * rewrite <- app_assoc; auto.
+      * rewrite <- app_assoc; auto.
+    + (* caller sem case *)
+      inv H1.
+      inv H7.
+      inv H1.
+      apply gamma_recognize__exists_gamma_derivation in H2.
+      destruct H2 as [vy hvy].
+      rewrite <- app_assoc.
+      eapply AFD_sem with (wmid' := wmid' ++ wpre)
+                          (v' := v' ++ [Node x vy]); eauto.
+      * rewrite <- app_assoc; auto.
+      * apply gamma_derivation_app; auto.
+        inv hw; rewrite app_nil_r in *.
+        rew_nil_r wmid; eauto.
+      * apply gamma_derivation_app; auto.
+        rew_nil_r wpre; eauto.
+      * repeat rewrite <- app_assoc; auto.
+      * unfold not; intros.
+        apply app_inj_tail in H; firstorder.
+    + inv H1.
+      rewrite <- app_assoc.
+      eapply AFD_tail; eauto.
+      * rewrite <- app_assoc; auto.
+      * apply gamma_derivation_app; auto.
+        inv hw; rewrite app_nil_r in *.
+        rew_nil_r wmid; eauto.
+Qed.
+
+Lemma consume_preserves_ambiguous_frames_derivation :
+  forall g fr fr' frs o pre suf v a l wpre wsuf,
+    fr = Fr (Loc o pre (T a :: suf)) v
+    -> fr' = Fr (Loc o (pre ++ [T a]) suf) (v ++ [Leaf a l])
+    -> ambiguous_frames_derivation g (fr :: frs) wpre ((a,l) :: wsuf)
+    -> ambiguous_frames_derivation g (fr' :: frs) (wpre ++ [(a,l)]) wsuf.
+Proof.
+  intros g fr fr' frs o pre suf v a l wpre wsuf ? ? ha; subst; inv ha.
+  - (* push case *)
+    inv H2.
+    rewrite <- app_assoc.
+    eapply AFD_push; eauto.
+    + rewrite <- app_assoc; auto.
+    + apply gamma_derivation_app; auto.
+      rew_nil_r ([(a,l)]); eauto.
+    + rewrite <- app_assoc; auto.
+    + rewrite <- app_assoc; auto.
+  - (* sem case *)
+    inv H1.
+    inv H5.
+    inv H1; sis.
+    rewrite <- app_assoc.
+    eapply AFD_sem with (wmid' := wmid' ++ [(a,l0)])
+                        (v' := v' ++ [Leaf a l0]); eauto.
+    + rewrite <- app_assoc; auto.
+    + apply gamma_derivation_app; auto.
+      rew_nil_r ([(a,l)]); eauto.
+    + apply gamma_derivation_app; auto.
+      rew_nil_r ([(a,l0)]); eauto.
+    + repeat rewrite <- app_assoc; auto.
+    + unfold not; intros.
+      apply app_inj_tail in H; destruct H; tc.
+  - inv H1.
+    rewrite <- app_assoc.
+    eapply AFD_tail; eauto.
+    + rewrite <- app_assoc; auto.
+    + apply gamma_derivation_app; auto.
+      rew_nil_r ([(a,l)]); eauto.
+Qed.
+
+Require Import GallStar.Prediction.
+
+Lemma allPredictionsEqual_false_exists_diff_rhs :
+  forall sp sps,
+    allPredictionsEqual sp sps = false
+    -> exists sp',
+      In sp' sps
+      /\ sp'.(prediction) <> sp.(prediction).
+Proof.
+  intros sp sps ha; unfold allPredictionsEqual in ha.
+  induction sps as [| sp' sps IH]; simpl in ha.
+  - inv ha.
+  - apply andb_false_iff in ha; destruct ha as [hh | ht].
+    + exists sp'; split.
+      * apply in_eq.
+      * unfold beqGamma in hh.
+        destruct (gamma_eq_dec sp.(prediction) sp'.(prediction)); inv hh; auto.
+    + apply IH in ht.
+      destruct ht as [sp'' [hi hn]].
+      exists sp''; split; auto.
+      apply in_cons; auto.
+Qed.
+
+(* refactor *)
+Lemma llPredict'_ambig_rhs_leads_to_successful_parse' :
+  forall g orig_sps wsuf wpre curr_sps rhs,
+    all_sp_stacks_wf g curr_sps
+    -> subparsers_sound_wrt_originals g orig_sps wpre curr_sps wsuf
+    -> llPredict' g curr_sps wsuf = PredAmbig rhs
+    -> exists orig_sp final_sp orig_sp' final_sp' rhs',
+        In orig_sp orig_sps
+        /\ orig_sp.(prediction) = rhs
+        /\ move_closure_multistep' g orig_sp (wpre ++ wsuf) final_sp []
+        /\ finalConfig final_sp = true
+        /\ In orig_sp' orig_sps
+        /\ orig_sp'.(prediction) = rhs'
+        /\ move_closure_multistep' g orig_sp' (wpre ++ wsuf) final_sp' []
+        /\ finalConfig final_sp' = true
+        /\ rhs' <> rhs.
+Proof.
+  intros g orig_sps wsuf.
+  induction wsuf as [| t wsuf' IH]; intros wpre curr_sps rhs ha hi hl; destruct curr_sps as [| csp csps]; sis; tc.
+  - destruct (allPredictionsEqual csp csps) eqn:ha'; tc.
+    unfold handleFinalSubparsers in hl.
+    destruct (filter _ _) as [| csp' csps'] eqn:hf; tc.
+    destruct (allPredictionsEqual csp' csps') eqn:ha''; tc.
+    inv hl.
+    unfold subparsers_sound_wrt_originals in hi.
+    pose proof hf as hf'.
+    eapply filter_cons_in in hf.
+    apply hi in hf.
+    destruct hf as [orig_sp [hi' hm]].
+    apply allPredictionsEqual_false_exists_diff_rhs in ha''.
+    destruct ha'' as [csp'' [hi'' hn]].
+    assert (hi''' : In csp'' (csp :: csps)).
+    { eapply filter_tail_in; eauto. }
+    apply hi in hi'''.
+    destruct hi''' as [orig_sp' [hi''' hm']].
+    exists orig_sp; exists csp'; exists orig_sp'; exists csp''; exists csp''.(prediction); repeat split; auto.
+    + (* easy *)
+      eapply mcms'_preserves_label; eauto.
+    + assert (hi'''' : In csp' (filter finalConfig (csp :: csps))).
+      { rewrite hf'; apply in_eq. }
+      eapply filter_In in hi''''; destruct hi''''; auto.
+    + eapply mcms'_preserves_label; eauto.
+    + assert (hi'''' : In csp'' (filter finalConfig (csp :: csps))).
+      { rewrite hf'; apply in_cons; auto. }
+      eapply filter_In in hi''''; destruct hi''''; auto.
+  - destruct (allPredictionsEqual _ _); tc.
+    destruct (move _ _ ) as [e | sps'] eqn:hm; tc.
+    destruct (closure _ _) as [e | sps''] eqn:hc; tc.
+    eapply IH with (wpre := wpre ++ [t]) in hl.
+    + destruct hl as [osp [fsp [osp' [fsp' [rhs' [hi' [heq [hm' [hf [hi'' [heq' [hm'' [hf' hn]]]]]]]]]]]]]; subst.
+      rewrite <- app_assoc in *; sis.
+      exists osp; exists fsp; exists osp'; exists fsp'; exists osp'.(prediction); repeat split; eauto.
+    + apply move_preserves_lstack_wf_invar in hm; auto.
+      apply closure_preserves_lstack_wf_invar in hc; auto.
+    + eapply move_closure_op_preserves_subparsers_sound_invar; eauto.
+Qed.
+
+(* okay, this version of the lemma is better because it doesn't
+   include unprocStackSyms in the conclusion *)
+Lemma llPredict_ambig_rhs_unproc_stack_syms' :
+  forall g cr ce o pre x suf frs w rhs,
+    cr = Loc o pre (NT x :: suf)
+    -> ce = Loc (Some x) [] rhs
+    -> no_left_recursion g
+    -> lstack_wf g (cr, frs)
+    -> llPredict g x (cr, frs) w = PredAmbig rhs
+    -> gamma_recognize g (rhs ++ suf ++ unprocTailSyms frs) w
+       /\ (exists rhs',
+              In (x, rhs') g
+              /\ rhs' <> rhs
+              /\ gamma_recognize g (rhs' ++ suf ++ unprocTailSyms frs) w).
+           
+Proof.
+  intros g cr ce o pre x suf frs w rhs ? ? hn hw hl; subst; sis.
+  pose proof hl as hl'; apply llPredict_ambig_in_grammar in hl'.
+  unfold llPredict in hl.
+  destruct (startState _ _ _) as [m | sps] eqn:hs; tc.
+  eapply llPredict'_ambig_rhs_leads_to_successful_parse'
+    with (orig_sps := sps) (wpre := []) in hl; sis.
+  - destruct hl as [osp [fsp [osp' [fsp' [rhs' [hi [heq [hm [hf [hi' [heq' [hm' [hf' hn']]]]]]]]]]]]]; subst.
+    split.
+    + eapply mcms'_final_config in hm; auto.
+      eapply closure_ussr_backwards with (sp' := osp) (w := w) in hs; eauto.
+      * destruct hs as [init_sp [hi'' [hc hg]]].
+      (* lemma? *)
+      unfold initSps in hi''.
+      apply in_map_iff in hi''.
+      destruct hi'' as [rhs [heq hi'']]; subst; sis.
+      apply closure_multistep_preserves_label in hc; sis; subst; auto.
+      * (* lemma *)
+        red. intros init_sp hi''.
+        eapply initSps_preserves_lstack_wf_invar; eauto.
+    + exists osp'.(prediction); repeat split; auto.
+      * eapply startState_sp_prediction_in_rhssForNt
+          with (sp' := osp') in hs; eauto.
+        apply rhssForNt_in_iff in hs; auto.
+      * eapply mcms'_final_config in hm'; auto.
+        eapply closure_ussr_backwards with (sp' := osp') (w := w) in hs; auto.
+        -- destruct hs as [init_sp [hi'' [hc hg]]].
+           (* lemma? *)
+           unfold initSps in hi''.
+           apply in_map_iff in hi''.
+           destruct hi'' as [rhs [heq hi'']]; subst; sis.
+           apply closure_multistep_preserves_label in hc; sis; subst; auto.
+        -- red; intros init_sp hi''.
+           eapply initSps_preserves_lstack_wf_invar; eauto.
+  - eapply stacks_wf_in_startState_result; eauto.
+    simpl; auto.
+  - red. intros sp' hi; sis.
+    exists sp'; split; auto.
+    eapply closure_func_refines_closure_multistep_backward in hi; eauto.
+    + destruct hi as [sp [hi hc]].
+      assert (hst : stable_config sp'.(stack)).
+      { eapply stable_config_after_closure_multistep; eauto. }
+      destruct sp' as [av pred ([o' pre' suf'], frs')]; sis.
+      inv hst; auto.
+    + red.
+      intros sp hi'.
+      eapply initSps_preserves_lstack_wf_invar; eauto.
+Qed.
+
+Definition ambiguous_prefix_derivation g w st :=
+  match st with
+  | Pst _ (fr, frs) wsuf u =>
+    u = false
+    -> exists wpre,
+        w = wpre ++ wsuf
+        /\ ambiguous_frames_derivation g (fr :: frs) wpre wsuf
+  end.
+
+Lemma apd_starts_true :
+  forall g ys ts,
+    ambiguous_prefix_derivation g ts (mkInitState g ys ts).
+Proof.
+  intros g ys ts.
+  unfold mkInitState; simpl.
+  intros hc; inv hc.
+Qed.
+
+Lemma step_preserves_apd :
+  forall g w st st',
+    no_left_recursion g
+    -> stack_wf g (Parser.stack st)
+    -> frames_prefix_derivation g w st
+    -> ambiguous_prefix_derivation g w st
+    -> step g st = StepK st'
+    -> ambiguous_prefix_derivation g w st'.
+Proof.
+  intros g w [av (fr,frs) wsuf u] [av' (fr',frs') wsuf' u'] hn hw hd ha hs.
+  red; red in ha.
+  intros hu.
+  unfold step in hs; dmeqs h; inv hs; tc.
+  - (* return *)
+    destruct ha as [wpre [heq ha]]; subst; sis; auto.
+    exists wpre; eapply return_preserves_ambiguous_frames_derivation in ha; eauto.
+  - (* consume *)
+    destruct ha as [wpre [heq ha]]; subst; sis; auto.
+    exists (wpre ++ [(t,l1)]); split; auto.
+    + apps.
+    + eapply consume_preserves_ambiguous_frames_derivation; eauto.
+  - (* unambiguous push *)
+    destruct ha as [wpre [heq ha]]; subst; sis; auto.
+    eexists; split; eauto.
+    rew_nil_r wpre.
+    eapply AFD_tail; eauto.
+  - (* ambiguous push *)
+    destruct u.
+    + (* u is true -- stack derivation is unique up to this point *)
+      red in hd.
+      destruct hd as [wpre [heq hd]]; subst.
+      exists wpre; split; auto.
+      clear ha.
+      rew_nil_r wpre.
+      eapply llPredict_ambig_rhs_unproc_stack_syms' in h4; eauto.
+      destruct h4 as [hr [rhs' [hi [hneq hr']]]].
+      eapply AFD_push; eauto.
+      simpl; auto.
+    + destruct ha as [wpre [heq ha]]; subst; sis; auto.
+      eexists; split; eauto.
+      rew_nil_r wpre.
+      eapply AFD_tail; eauto.
+Qed.
+
+Lemma multistep_sound_ambig' :
+  forall (g      : grammar)
+         (tri    : nat * nat * nat)
+         (a      : Acc lex_nat_triple tri)
+         (w wsuf : list token)
+         (av     : NtSet.t)
+         (stk    : parser_stack)
+         (u      : bool)
+         (a'     : Acc lex_nat_triple (Parser.meas g (Pst av stk wsuf u)))
+         (v      : forest),
+    tri = Parser.meas g (Pst av stk wsuf u)
+    -> no_left_recursion g
+    -> stack_wf g stk
+    -> frames_prefix_derivation g w (Pst av stk wsuf u)
+    -> ambiguous_prefix_derivation g w (Pst av stk wsuf u)
+    -> multistep g (Pst av stk wsuf u) a' = Ambig v
+    -> gamma_derivation g (bottomFrameSyms stk) w v
+       /\ (exists v',
+              gamma_derivation g (bottomFrameSyms stk) w v'
+              /\ v' <> v).
+Proof.
+  intros g tri a.
+  induction a as [tri hlt IH].
+  intros w wsuf av stk u a' v heq hn hw hf hi hm; subst.
+  apply multistep_ambig_cases in hm.
+  destruct hm as [[hs hu] | he].
+  - simpl in hu; subst.
+    apply step_StepAccept_facts in hs.
+    destruct hs as [[xo [rpre [v' [heq]]]] heq']; subst.
+    unfold bottomFrameSyms; simpl; rewrite app_nil_r.
+    red in hi.
+    destruct hi as [wpre [heq ha]]; subst; auto.
+    clear IH. clear a'. clear hlt.
+    inv ha.
+    + inv H1; sis. unfold unprocTailSyms' in *; sis.
+      rewrite app_nil_r in *; subst.
+      inv H2; sis.
+      inv H5; sis.
+      rewrite app_nil_r in *. 
+      firstorder.
+    + inv H2.
+  - destruct he as [st' [a'' [hf' hm]]].
+    destruct st' as [av' stk' wsuf'].
+    eapply IH with (w := w) in hm; eauto. 
+    + erewrite step_preserves_bottomFrameSyms_invar; eauto.
+    + apply step_meas_lt; auto.
+    + eapply step_preserves_stack_wf_invar; eauto.
+    + eapply step_preserves_frames_prefix_derivation; eauto.
+      simpl; auto.
+    + eapply step_preserves_apd; eauto.
+      simpl; auto.
+Qed.
+
+Lemma multistep_sound_ambig :
+  forall (g      : grammar)
+         (w wsuf : list token)
+         (av     : NtSet.t)
+         (stk    : parser_stack)
+         (u      : bool)
+         (a      : Acc lex_nat_triple (Parser.meas g (Pst av stk wsuf u)))
+         (v      : forest),
+    no_left_recursion g
+    -> stack_wf g stk
+    -> frames_prefix_derivation g w (Pst av stk wsuf u)
+    -> ambiguous_prefix_derivation g w (Pst av stk wsuf u)
+    -> multistep g (Pst av stk wsuf u) a = Ambig v
+    -> gamma_derivation g (bottomFrameSyms stk) w v
+       /\ (exists v',
+              gamma_derivation g (bottomFrameSyms stk) w v'
+              /\ v' <> v).
+Proof.
+  intros; eapply multistep_sound_ambig'; eauto.
+Qed.
+
+Theorem parse_sound_ambig :
+  forall (g  : grammar)
+         (ys : list symbol)
+         (ts : list token)
+         (v  : forest),
+    no_left_recursion g
+    -> parse g ys ts = Ambig v
+    -> gamma_derivation g ys ts v
+       /\ (exists v',
+              gamma_derivation g ys ts v'
+              /\ v' <> v).
+Proof.
+  intros g ys ts v hn hp.
+  unfold parse in hp.
+  eapply multistep_sound_ambig in hp; eauto.
+  - constructor.
+  - (* lemma *)
+    red.
+    exists []; split; eauto.
+    rew_nil_r ([] : list token); eauto.
+  - apply apd_starts_true.
+Qed.
+Print Assumptions parse_sound_ambig.
